todo.md
@@ -1,0 +1,7 @@
+
+
+# Todo #
+
+    * tactic for monotonicity in predicate calculus
+    * reduce soundness of leads-to properties to assumptions about transient
+	* prove soundness of unitb.models.sched
